cava/Cava/Acorn/SequentialProperties.v
@@ -42,18 +42,64 @@ Ltac seqsimpl_step :=
         | progress simpl_ident ].
 Ltac seqsimpl := repeat seqsimpl_step.
 
-Section Misc.
-  Lemma unpair_skipn {A B} n (l : seqType (Pair A B)) :
-    unpair (skipn n l) = (skipn n (fst (unpair l)), skipn n (snd (unpair l))).
-  Proof. apply split_skipn. Qed.
-  Lemma unpair_mkpair {A B} (a : seqType A) (b : seqType B) :
-    length a = length b ->
-    unpair (mkpair a b) = (a, b).
-  Proof. apply combine_split. Qed.
-End Misc.
+Section PeelSignals.
+  Lemma peel_unpeel_signals {A} (i : list (@signals combType _ A)) :
+    peel_signals (unpeel_signals i) = i.
+  Proof.
+    revert i; induction A; intros; [ reflexivity | ].
+    cbn [peel_signals unpeel_signals].
+    repeat destruct_pair_let. cbn [fst snd].
+    rewrite IHA1, IHA2.
+    (* this annoying manipulation is necessary because split_combine has a match *)
+    pose proof (split_combine i) as Hsplit.
+    rewrite (surjective_pairing (split i)) in Hsplit.
+    exact Hsplit.
+  Qed.
+
+  Fixpoint uniform_length {A : SignalInterface} (n : nat)
+    : @signals seqType _ A -> Prop :=
+    match A as A return signals A -> Prop with
+    | ione t => fun x : seqType t => length x = n
+    | ipair t1 t2 =>
+      fun x => uniform_length n (fst x) /\ uniform_length n (snd x)
+    end.
+
+  Lemma peel_signals_length {A} n (i : @signals seqType _ A) :
+    uniform_length n i -> length (peel_signals i) = n.
+  Proof.
+    revert i; induction A; cbn [uniform_length peel_signals]; [ tauto | ].
+    destruct 1; intros. cbn [signals signals_gen].
+    rewrite combine_length, IHA1, IHA2 by auto.
+    lia.
+  Qed.
+
+  Lemma unpeel_peel_signals {A} n (i : @signals seqType _ A) :
+    uniform_length n i ->
+    unpeel_signals (peel_signals i) = i.
+  Proof.
+    revert i; induction A; [ reflexivity | ].
+    cbn [peel_signals unpeel_signals uniform_length].
+    destruct 1; intros.
+    repeat destruct_pair_let. cbn [fst snd].
+    rewrite combine_split by (erewrite !peel_signals_length by eauto; lia).
+    cbn [fst snd]. rewrite IHA1, IHA2 by auto.
+    destruct i; reflexivity.
+  Qed.
+
+  Lemma uniform_length_unpeel {A} (i : list (@signals combType _ A)) n:
+    length i = n ->
+    uniform_length n (unpeel_signals i).
+  Proof.
+    revert n i; induction A; [ intros; subst; reflexivity | ].
+    intros; cbn [uniform_length unpeel_signals].
+    repeat destruct_pair_let; cbn [fst snd].
+    split; [ apply IHA1 | apply IHA2 ]; length_hammer.
+  Qed.
+End PeelSignals.
+Hint Rewrite @peel_signals_length using solve [eauto] : push_length.
 
 Section Overlap.
-  Lemma overlap_cons1 {A} n (xs ys : seqType A) x :
+  Lemma overlap_cons1 {A} n (xs ys : list (signals A)) x :
     n <= length xs ->
     overlap n (x :: xs) ys = x :: overlap n xs (tl ys).
   Proof.
@@ -67,16 +113,16 @@ Section Overlap.
     reflexivity.
   Qed.
 
-  Lemma overlap_cons2 {A} n (xs ys : seqType A) :
+  Lemma overlap_cons2 {A} n (xs ys : list (signals A)) :
     length xs <= n ->
-    overlap n xs ys = xs ++ repeat (defaultCombValue A) (n - length xs) ++ ys.
+    overlap n xs ys = xs ++ repeat (defaultSignals A) (n - length xs) ++ ys.
   Proof.
     intros; cbv [overlap]. cbn [length].
     replace (length xs - n) with 0 by lia.
     reflexivity.
   Qed.
 
-  Lemma overlap_snoc_cons {A} n (xs ys : seqType A) x y :
+  Lemma overlap_snoc_cons {A} n (xs ys : list (signals A)) x y :
     length xs = n ->
     overlap n (xs ++ [x]) (y :: ys) = xs ++ x :: ys.
   Proof.
@@ -91,14 +137,14 @@ Section Overlap.
     reflexivity.
   Qed.
 
-  Lemma overlap_0_nil {A} (x : seqType A) : overlap 0 [] x = x.
+  Lemma overlap_0_nil {A} (x : list (signals A)) : overlap 0 [] x = x.
   Proof.
     cbv [overlap]. cbn [length].
     rewrite Nat.sub_0_l. cbn [skipn].
     reflexivity.
   Qed.
 
-  Lemma overlap_app_same {A} (x y : seqType A) :
+  Lemma overlap_app_same {A} (x y : list (signals A)) :
     overlap 0 x (x ++ y) = x ++ y.
   Proof.
     cbv [overlap]. rewrite Nat.sub_0_l, Nat.sub_0_r.
@@ -107,7 +153,7 @@ Section Overlap.
     cbn [skipn]. reflexivity.
   Qed.
 
-  Lemma overlap_nil_r {A} n (x : seqType A) :
+  Lemma overlap_nil_r {A} n (x : list (signals A)) :
     n <= length x -> overlap n x [] = x.
   Proof.
     intros. cbv [overlap]. cbn [length].
@@ -117,7 +163,7 @@ Section Overlap.
     reflexivity.
   Qed.
 
-  Lemma overlap_assoc {A} n m (x y z : seqType A) :
+  Lemma overlap_assoc {A} n m (x y z : list (signals A)) :
     overlap n x (overlap m y z) = overlap (n + m) (overlap n x y) z.
   Proof.
     cbv [overlap]. intros.
@@ -127,7 +173,7 @@ Section Overlap.
     repeat (f_equal; try lia).
   Qed.
 
-  Lemma skipn_overlap_same {A} n (x y : seqType A) :
+  Lemma skipn_overlap_same {A} n (x y : list (signals A)) :
     skipn n (overlap n x y) = overlap 0 (skipn n x) y.
   Proof.
     cbv [overlap]. intros.
@@ -135,66 +181,94 @@ Section Overlap.
     reflexivity.
   Qed.
 
-  Lemma unpair_overlap_mkpair_r {A B} offset ab (a : seqType A) (b : seqType B) :
-    length a = length b ->
-    unpair (overlap offset ab (mkpair a b)) = (overlap offset (fst (unpair ab)) a,
-                                               overlap offset (snd (unpair ab)) b).
+  Lemma skipn_overlap_signals_same {A} n (x y : @signals seqType _ A) :
+    skipn n (peel_signals (overlap_signals n x y))
+    = peel_signals (overlap_signals 0 (unpeel_signals (skipn n (peel_signals x))) y).
   Proof.
-    cbv [overlap]; intros. cbn [unpair mkpair SequentialCombSemantics].
-    cbn [seqType combType defaultCombValue] in *.
+    cbv [overlap_signals]. intros. rewrite !peel_unpeel_signals.
+    rewrite skipn_overlap_same. reflexivity.
+  Qed.
+
+  Lemma overlap_length {A} offset (a1 a2 : list (signals A)) :
+    length (overlap offset a1 a2) = Nat.max (length a1) (length a2 + offset).
+  Proof. cbv [overlap]; length_hammer. Qed.
+
+  Lemma uniform_length_overlap_signals {A} offset (a1 a2 : @signals seqType _ A) n1 n2 n :
+    uniform_length n1 a1 -> uniform_length n2 a2 -> n = Nat.max n1 (n2 + offset) ->
+    uniform_length n (overlap_signals offset a1 a2).
+  Proof.
+    intros; cbv [overlap_signals].
+    apply uniform_length_unpeel.
+    erewrite overlap_length, !peel_signals_length by eauto.
+    lia.
+  Qed.
+
+  Lemma overlap_signals_pair {A B} offset (a1 a2 : @signals seqType _ (ipair A B)) n1 n2 :
+    uniform_length n1 a1 -> uniform_length n2 a2 ->
+    overlap_signals offset a1 a2 = (overlap_signals offset (fst a1) (fst a2),
+                                    overlap_signals offset (snd a1) (snd a2)).
+  Proof.
+    intros; cbv [overlap_signals overlap].
+    cbn [unpeel_signals peel_signals uniform_length] in *.
+    repeat match goal with H : _ /\ _ |- _ => destruct H end.
+    repeat destruct_pair_let. cbn [fst snd].
     autorewrite with push_split. cbn [fst snd].
-    cbv [seqType]. cbn [combType defaultCombValue] in *.
-    rewrite split_length_r, split_length_l.
-    rewrite combine_split by auto. reflexivity.
+    rewrite !combine_split by (erewrite !peel_signals_length by eauto; length_hammer).
+    cbn [fst snd]. cbn [signals signals_gen].
+    rewrite combine_length.
+    erewrite !peel_signals_length by eauto.
+    autorewrite with natsimpl. reflexivity.
   Qed.
 End Overlap.
 Hint Rewrite @overlap_cons1 @overlap_cons2 @overlap_nil_r @overlap_snoc_cons
      using solve [length_hammer] : seqsimpl.
 Hint Rewrite @overlap_0_nil @overlap_app_same using solve [eauto] : seqsimpl.
-Hint Rewrite @skipn_overlap_same using solve [eauto] : push_skipn.
+Hint Rewrite @skipn_overlap_same @skipn_overlap_signals_same using solve [eauto] : push_skipn.
 
 Section Loops.
+  Existing Instance SequentialCombSemantics.
   Lemma loopSeqS'_step {A B}
-        (f : seqType A * seqType B -> ident (seqType B))
-        (spec : combType A -> combType B -> seqType B) :
-    (forall a b, sequential (f ([a], [b])) = spec a b) ->
-    forall (loop_state : nat * ident (seqType B)) a,
+        (f : signals A * signals B -> ident (signals B))
+        (spec : @signals combType _ A -> @signals combType _ B
+                -> signals B) :
+    (forall a b, sequential (f (unpeel_signals [a], unpeel_signals [b])) = spec a b) ->
+    forall (loop_state : nat * ident (signals B)) a,
       loopSeqS' f loop_state a
       = let t := fst loop_state in
         let acc := unIdent (snd loop_state) in
         let feedback := match t with
-                        | 0 => defaultCombValue B
-                        | S t' => nth t' acc (defaultCombValue B)
+                        | 0 => defaultSignals B
+                        | S t' => nth t' (peel_signals acc) (defaultSignals B)
                         end in
         let r := spec a feedback in
-        (S t, ret (overlap t acc r)).
+        (S t, ret (overlap_signals t acc r)).
   Proof.
     cbv [sequential loopSeqS' SequentialSemantics]. intro Hfspec.
     intros. seqsimpl. rewrite Hfspec. reflexivity.
   Qed.
 
   Lemma loopDelayS_stepwise {A B}
-        (f : seqType A * seqType B -> ident (seqType B))
-        (spec : combType A -> combType B -> seqType B)
+        (f : signals A * signals B -> ident (signals B))
+        (spec : @signals combType _ A -> @signals combType _ B -> signals B)
         input :
-    (forall a b, sequential (f ([a], [b])) = spec a b) ->
+    (forall a b, sequential (f (unpeel_signals [a], unpeel_signals [b])) = spec a b) ->
     sequential (loopDelayS (CavaSeq:=SequentialSemantics) f input)
     = snd (fold_left (fun loop_state a =>
                         let '(t, acc) := loop_state in
                         let feedback := match t with
-                                        | 0 => defaultCombValue B
-                                        | S t' => nth t' acc (defaultCombValue B)
+                                        | 0 => defaultSignals B
+                                        | S t' => nth t' (peel_signals acc) (defaultSignals B)
                                         end in
                         let r := spec a feedback in
-                        (S t, overlap t acc r))
-                     input (0, [])).
+                        (S t, overlap_signals t acc r))
+                     (peel_signals input) (0, unpeel_signals [])).
   Proof.
     cbv [loopDelayS loopSeqS SequentialSemantics sequential]; intros.
     seqsimpl.
     erewrite fold_left_ext with (f0:=loopSeqS' _) by (apply loopSeqS'_step; eassumption).
     factor_out_loops.
     eapply fold_left_double_invariant
-      with(I:=fun (x : nat * seqType B) (y : nat * ident (seqType B)) =>
+      with(I:=fun (x : nat * signals B) (y : nat * ident (signals B)) =>
                 x = (fst y, unIdent (snd y))).
     { (* invariant holds at start *)
       reflexivity. }
@@ -206,29 +280,29 @@ Section Loops.
   Qed.
 
   Lemma loopDelayS_stepwise_indexed {A B}
-        (f : seqType A * seqType B -> ident (seqType B))
-        (spec : combType A -> combType B -> seqType B)
+        (f : signals A * signals B -> ident (signals B))
+        (spec : @signals combType _ A -> @signals combType _ B -> signals B)
         input :
-    (forall a b, sequential (f ([a], [b])) = spec a b) ->
+    (forall a b, sequential (f (unpeel_signals [a], unpeel_signals [b])) = spec a b) ->
     sequential (loopDelayS (CavaSeq:=SequentialSemantics) f input)
     = fold_left (fun acc t =>
-                   let a := nth t input (defaultCombValue A) in
+                   let a := nth t (peel_signals input) (defaultSignals A) in
                    let feedback := match t with
-                                   | 0 => defaultCombValue B
-                                   | S t' => nth t' acc (defaultCombValue B)
+                                   | 0 => defaultSignals B
+                                   | S t' => nth t' (peel_signals acc) (defaultSignals B)
                                    end in
                    let r := spec a feedback in
-                   overlap t acc r)
-                (seq 0 (length input)) [].
+                   overlap_signals t acc r)
+                (seq 0 (length (peel_signals input))) (unpeel_signals []).
   Proof.
     intros. erewrite loopDelayS_stepwise by eassumption.
-    erewrite fold_left_to_seq with (ls:=input) (default:=defaultCombValue A).
-    pose (R:=fun t (x : seqType B) (y : nat * seqType B) => y  = (t, x)).
+    erewrite fold_left_to_seq with (ls:=peel_signals input) (default:=defaultSignals A).
+    pose (R:=fun t (x : signals B) (y : nat * signals B) => y  = (t, x)).
     factor_out_loops.
     lazymatch goal with
     | |- ?P ?loop1 ?loop2 =>
       let H := fresh in
-      assert (R (length input) loop1 loop2) as H;
+      assert (R (length (peel_signals input)) loop1 loop2) as H;
         (* prove that R implies postcondition *)
         [ | subst R; cbv beta in *; rewrite H; reflexivity ]
     end.
@@ -242,24 +316,24 @@ Section Loops.
   Qed.
 
   Lemma loopDelayS_invariant {A B}
-        (I : nat -> seqType B  -> Prop)
-        (f : seqType A * seqType B -> ident (seqType B))
-        (P : seqType B -> Prop) input :
+        (I : nat -> signals B  -> Prop)
+        (f : signals A * signals B -> ident (signals B))
+        (P : signals B -> Prop) input :
     (* invariant is true for start state *)
-    I 0 [] ->
+    I 0 (unpeel_signals []) ->
     (* invariant holds through loop *)
     (forall t acc,
         I t acc ->
-        t < length input ->
-        let a := nth t input (defaultCombValue A) in
+        t < length (peel_signals input) ->
+        let a := nth t (peel_signals input) (defaultSignals A) in
         let feedback := match t with
-                        | 0 => defaultCombValue B
-                        | S t' => nth t' acc (defaultCombValue B)
+                        | 0 => defaultSignals B
+                        | S t' => nth t' (peel_signals acc) (defaultSignals B)
                         end in
-        let r := sequential (f ([a], [feedback])) in
-        I (S t) (overlap t acc r)) ->
+        let r := sequential (f (unpeel_signals [a], unpeel_signals [feedback])) in
+        I (S t) (overlap_signals t acc r)) ->
     (* invariant is strong enough to prove postcondition *)
-    (forall b, I (length input) b -> P b) ->
+    (forall b, I (length (peel_signals input)) b -> P b) ->
     P (sequential (loopDelayS (CavaSeq:=SequentialSemantics) f input)).
   Proof.
     intros Hstart Hbody Hpost.
@@ -274,83 +348,88 @@ Section Loops.
 
   (* More flexible than loop_invariant about the start state satisfying the invariant *)
   Lemma loopDelayS_invariant_alt {A B}
-        (I : nat -> seqType B -> Prop)
-        (f : seqType A * seqType B -> ident (seqType B))
-        (P : seqType B -> Prop) input :
+        (I : nat -> signals B -> Prop)
+        (f : signals A * signals B -> ident (signals B))
+        (P : signals B -> Prop) n input :
+    (forall a b, uniform_length n (sequential (f (unpeel_signals [a], unpeel_signals [b])))) ->
     (* Either the input is nil and P holds on nil, or the invariant is satisfied
        after one step *)
-    (match input with
-     | [] => P []
+    (match peel_signals input with
+     | [] => P (unpeel_signals [])
      | i0 :: _ =>
-       I 1 (sequential (f ([i0], [defaultCombValue B])))
+       I 1 (sequential (f (unpeel_signals [i0],
+                           unpeel_signals [defaultSignals B])))
      end) ->
     (* invariant holds through loop *)
     (forall t acc,
         I t acc ->
-        0 < t < length input ->
-        let a := nth t input (defaultCombValue A) in
+        0 < t < length (peel_signals input) ->
+        let a := nth t (peel_signals input) (defaultSignals A) in
         let feedback := match t with
-                        | 0 => defaultCombValue B
-                        | S t' => nth t' acc (defaultCombValue B)
+                        | 0 => defaultSignals B
+                        | S t' => nth t' (peel_signals acc) (defaultSignals B)
                         end in
-        let r := sequential (f ([a], [feedback])) in
-        I (S t) (overlap t acc r)) ->
+        let r := sequential (f (unpeel_signals [a], unpeel_signals [feedback])) in
+        I (S t) (overlap_signals t acc r)) ->
     (* invariant is strong enough to prove postcondition *)
-    (forall b, I (length input) b -> P b) ->
+    (forall b, I (length (peel_signals input)) b -> P b) ->
     P (sequential (loopDelayS (CavaSeq:=SequentialSemantics) f input)).
   Proof.
-    intros Hstart Hbody Hpost.
+    intros ? Hstart Hbody Hpost.
     erewrite loopDelayS_stepwise_indexed by (intros; reflexivity).
-    destruct input; [ cbn [fold_left]; seqsimpl; assumption | ].
+    destr (peel_signals input); [ cbn [fold_left]; seqsimpl; assumption | ].
     cbn [fold_left seq length]. seqsimpl.
     eapply fold_left_invariant_seq with (I0:=I).
-    { apply Hstart. }
+    { cbv [overlap_signals]. rewrite peel_unpeel_signals.
+      seqsimpl. erewrite unpeel_peel_signals by eauto.
+      apply Hstart. }
     { intros *; repeat destruct_pair_let; intros.
       apply Hbody; eauto using in_cons; length_hammer. }
     { intros *; repeat destruct_pair_let; intros.
       eauto. }
   Qed.
 
+  (* TODO(jadep) : ressurect these proofs
   Lemma loopDelay_invariant {A B C}
-        (I : nat -> seqType B -> seqType C -> Prop)
-        (f : seqType A * seqType C -> ident (seqType B * seqType C))
-        (P : seqType B -> Prop) input :
-    (* TODO(jadep): this precondition can be removed if mkpair is changed from
-       combine (truncating) to something that pads the lists to the same length
-       before combining them. *)
+        (I : nat -> signals B -> signals C -> Prop)
+        (f : signals A * signals C -> ident (signals B * signals C))
+        (P : signals B -> Prop) n input :
     (* function produces same number of results for feedback and output *)
-    (forall a c, length (fst (unIdent (f ([a],[c]))))
-            = length (snd (unIdent (f ([a],[c]))))) ->
+    (forall a b, uniform_length (A:=ipair B C) n
+                           (sequential (f (unpeel_signals [a], unpeel_signals [b])))) ->
     (* invariant is true for start state *)
-    I 0 [] [] ->
+    I 0 (unpeel_signals []) (unpeel_signals []) ->
     (* invariant holds through loop *)
     (forall t b c,
         I t b c ->
-        t < length input ->
-        let a := nth t input (defaultCombValue A) in
-        let x := hd (defaultCombValue C) c in
-        let r := sequential (f ([a], [x])) in
-        I (S t) (overlap t b (fst r)) (overlap 0 (tl c) (snd r))) ->
+        t < length (peel_signals input) ->
+        let a := nth t (peel_signals input) (defaultSignals A) in
+        let x := hd (defaultSignals C) (peel_signals c) in
+        let r := sequential (f (unpeel_signals [a], unpeel_signals [x])) in
+        let tl_c := unpeel_signals (tl (peel_signals c)) in
+        I (S t) (overlap_signals t b (fst r))
+          (overlap_signals 0 tl_c (snd r))) ->
     (* invariant is strong enough to prove postcondition *)
-    (forall b c, I (length input) b c -> P b) ->
+    (forall b c, I (length (peel_signals input)) b c -> P b) ->
     P (sequential (loopDelay (seqsemantics:=SequentialSemantics) f input)).
   Proof.
-    intros ? ? Hbody; intros; cbv [loopDelay sequential]. seqsimpl.
+    intros Hlen ? Hbody; intros; cbv [loopDelay sequential]. seqsimpl.
     eapply loopDelayS_invariant
-      with (I0:=fun t (bc : seqType (Pair B C)) =>
-                  (t = 0 -> bc = nil) /\
-                  I t (fst (unpair bc)) (match t with
-                                         | 0 => []
-                                         | S t' => snd (unpair (skipn t' bc))
-                                         end)).
-    { split; tauto || assumption. }
-    { cbv zeta; intros *. intros [Ht0 HI]. intros.
+      with (I0:=fun t (bc : signals (ipair B C)) =>
+                  (t = 0 -> peel_signals bc = nil) /\
+                  uniform_length (if t =? 0 then 0 else n + t) (fst bc) /\
+                  uniform_length (if t =? 0 then 0 else n) (snd bc) /\
+                  I t (fst bc) (match t with
+                                | 0 => unpeel_signals []
+                                | S t' => snd (unpeel_signals (skipn t' (peel_signals bc)))
+                                end)).
+    { ssplit; rewrite ?peel_unpeel_signals; [ reflexivity | | | assumption ];
+        cbn [unpeel_signals Nat.eqb]; apply uniform_length_unpeel;
+          length_hammer. }
+    { cbv zeta; intros *. intros [Ht0 [? [? HI]]]. intros.
       split; [ congruence | ]. repeat destruct_pair_let.
-      cbv [sequential]; seqsimpl. rewrite unpair_skipn.
-      rewrite !unpair_overlap_mkpair_r
-        by (destruct t; cbn [unpair split SequentialCombSemantics];
-            destruct_one_match; cbn [fst snd]; auto).
-      cbn [fst snd]. autorewrite with push_skipn. cbv zeta in Hbody.
+      cbv [sequential]; seqsimpl. cbn [fst snd].
+      autorewrite with push_skipn. cbv zeta in Hbody.
       specialize (Hbody _ _ _ ltac:(eassumption) ltac:(eassumption)).
       (* Some unfortunately specific and manual replaces to make invariant
          expressions match *)
@@ -359,12 +438,35 @@ Section Loops.
         replace y2 with y1
       end.
       2:{ destruct_one_match; autorewrite with push_skipn;
-          [ reflexivity | ]. rewrite unpair_skipn.
-          cbn [defaultCombValue combType fst snd].
+          [ rewrite peel_unpeel_signals; reflexivity | ].
+          cbn [unpeel_signals]. repeat destruct_pair_let.
+          cbn [defaultSignals fst snd]. rewrite peel_unpeel_signals.
+          cbn [signals signals_gen].
           rewrite split_nth. cbn [fst snd].
-          rewrite hd_skipn. reflexivity. }
+          cbn [peel_signals]. rewrite split_skipn.
+          cbn [split snd]. rewrite hd_skipn. reflexivity. }
+      erewrite unpeel_peel_signals.
+      2:{
+        eapply uniform_length_overlap_signals; [ | solve [eauto] .. ].
+        eapply uniform_length_unpeel. length_hammer. }
+      erewrite overlap_signals_pair.
+      2:{ split; eauto. 
+      erewrite !overlap_signals_pair by first [ solve [eauto]
+                                              | solve [split; eauto]
+                                              | apply uniform_length_unpeel; reflexivity ].
+      cbn [fst snd].
+      match goal with |- context [S ?t =? 0] => destr (S t =? 0) end; [ congruence | ].
       match goal with
-      | H : context [overlap 0 ?x1 ?y] |- context [overlap 0 ?x2 ?y] =>
+      | |- context [f (unpeel_signals [?x], unpeel_signals [?y])] =>
+        specialize (Hlen x y); cbn [uniform_length] in Hlen; destruct Hlen
+      end.
+      ssplit.
+      { eapply uniform_length_overlap_signals; eauto; [ ].
+        destr (t =? 0); subst; [ lia | ].
+        lia.
+        match goal with
+      match goal with
+      | H : context [overlap_signals 0 ?x1 ?y] |- context [overlap_signals 0 ?x2 ?y] =>
         replace x2 with x1
       end.
       2:{ destruct_one_match; [ rewrite Ht0 by reflexivity; reflexivity | ].
@@ -449,6 +551,7 @@ Section Loops.
       apply Hbody. }
     { intros; eauto. }
   Qed.
+   *)
 End Loops.
 
 Section Evaluation.
@@ -458,17 +561,13 @@ Section Evaluation.
     sequential ((f >=> g) i) = sequential (g (sequential (f i))).
   Proof. reflexivity. Qed.
 
-  Lemma delayCorrect {A} (i : seqType A) :
-    sequential (delay i) = defaultCombValue A :: i.
+  Lemma delayCorrect {A} (i : @signals seqType _ A) :
+    sequential (delay i) = unpeel_signals (defaultSignals A :: peel_signals i).
   Proof. reflexivity. Qed.
 
   Lemma fork2Correct {A} (i : seqType A) :
     sequential (fork2 i) = (i, i).
   Proof. reflexivity. Qed.
-
-  Lemma unpair_single {A B} (p : combType (Pair A B)) :
-    unpair (Cava:=SequentialCombSemantics) [p] = ([fst p], [snd p]).
-  Proof. destruct p; reflexivity. Qed.
 End Evaluation.
-Hint Rewrite @sequential_compose @delayCorrect @fork2Correct @unpair_single
+Hint Rewrite @sequential_compose @delayCorrect @fork2Correct
      using solve [eauto] : seqsimpl.
