cava/Cava/Acorn/Identity.v
@@ -29,8 +29,10 @@ Existing Instance CombinationalSemantics.
 
 (* Lemmas about combinators specialized to the identity monad *)
 Section Combinators.
-  Lemma zipWith_unIdent {A B C : SignalType} n f va vb :
-    unIdent (@zipWith _ _ Monad_ident A B C n f va vb)
+  Lemma zipWith_unIdent {A B C : SignalType} n f
+        (va : Vector.t (combType A) n) (vb : Vector.t (combType B) n) :
+    @unIdent (Vector.t (combType C) n)
+             (@zipWith _ _ Monad_ident A B C n f va vb)
     = map2 (fun a b => unIdent (f (a,b))) va vb.
   Proof.
     cbv [zipWith Traversable.mapT Traversable_vector].
@@ -67,10 +69,4 @@ Hint Rewrite @zipWith_unIdent @xorV_unIdent
 Ltac simpl_ident :=
   repeat
     first [ progress autorewrite with simpl_ident
-          | erewrite map2_ext; [ | intros; progress simpl_ident;
-                                   instantiate_app_by_reflexivity ]
-          | erewrite map_ext; [ | intros; progress simpl_ident;
-                                  instantiate_app_by_reflexivity ]
-          | erewrite fold_left_ext; [ | intros; progress simpl_ident;
-                                        instantiate_app_by_reflexivity ]
           | progress cbn [fst snd bind ret Monad_ident unIdent] ].
